backend/RTLtyping_old.v
@@ -186,7 +186,7 @@ Inductive wt_fundef: fundef -> Prop :=
       wt_fundef (Internal f).
 
 Definition wt_program (p: program): Prop :=
-  forall i f, In (i, Gfun f) (prog_defs p) -> wt_fundef f.
+  forall i f, In (i, Some (Gfun f)) (prog_defs p) -> wt_fundef f.
 
 (** * Type inference *)
 
@@ -824,6 +824,9 @@ Proof.
   apply wt_regset_assign; auto.
 Qed.
 
+Section WITHEXTCALLS.
+Context `{external_calls_prf: ExternalCalls}.
+
 Lemma wt_exec_Iop:
   forall (ge: genv) env f sp op args res s rs m v,
   wt_instr f env (Iop op args res s) ->
@@ -868,9 +871,12 @@ Proof.
   intros. inv H. eauto.
 Qed.
 
+Section WITHRESTYP.
+Variable (restyp: option typ).
+
 Inductive wt_stackframes: list stackframe -> signature -> Prop :=
   | wt_stackframes_nil: forall sg,
-      sg.(sig_res) = Some Tint ->
+      Some sg.(sig_res) = Some restyp ->
       wt_stackframes nil sg
   | wt_stackframes_cons:
       forall s res f sp pc rs env sg,
@@ -888,11 +894,11 @@ Inductive wt_state: state -> Prop :=
         (WT_RS: wt_regset env rs),
       wt_state (State s f sp pc rs m)
   | wt_state_call:
-      forall s f args m (*SACC:*)sz,
+      forall s f args m sz,
       wt_stackframes s (funsig f) ->
       wt_fundef f ->
       Val.has_type_list args (sig_args (funsig f)) ->
-      wt_state (Callstate s f args m (*SACC:*)sz)
+      wt_state (Callstate s f args m sz)
   | wt_state_return:
       forall s v m sg,
       wt_stackframes s sg ->
@@ -908,6 +914,8 @@ Proof.
 - econstructor; eauto. rewrite H3. unfold proj_sig_res. rewrite H. auto.
 Qed.
 
+End WITHRESTYP.
+
 Section SUBJECT_REDUCTION.
 
 Variable p: program.
@@ -916,73 +924,71 @@ Hypothesis wt_p: wt_program p.
 
 Let ge := Genv.globalenv p.
 
-(*SACC:*)
-Variable fn_stack_requirements : ident -> Z.
+Variable restyp: option typ.
+
+Variable fn_stack_requirements: ident -> Z.
 
 Lemma subject_reduction:
-  forall st1 t st2, step (*SACC:*)fn_stack_requirements ge st1 t st2 ->
-  forall (WT: wt_state st1), wt_state st2.
+  forall st1 t st2, step fn_stack_requirements ge st1 t st2 ->
+  forall (WT: wt_state restyp st1), wt_state restyp st2.
 Proof.
   induction 1; intros; inv WT;
   try (generalize (wt_instrs _ _ WT_FN pc _ H); intros WTI).
-- (* Inop *)
+  (* Inop *)
   econstructor; eauto.
-- (* Iop *)
+  (* Iop *)
   econstructor; eauto. eapply wt_exec_Iop; eauto.
-- (* Iload *)
+  (* Iload *)
   econstructor; eauto. eapply wt_exec_Iload; eauto.
-- (* Istore *)
+  (* Istore *)
   econstructor; eauto.
-- (* Icall *)
+  (* Icall *)
   assert (wt_fundef fd).
-  { destruct ros; simpl in H1.
+    destruct ros; simpl in H0.
     pattern fd. apply Genv.find_funct_prop with fundef unit p (rs#r).
-    exact wt_p. exact H1.
-    caseEq (Genv.find_symbol ge i); intros. rewrite H2 in H1.
+    exact wt_p. exact H0.
+    caseEq (Genv.find_symbol ge i); intros; rewrite H1 in H0.
     pattern fd. apply Genv.find_funct_ptr_prop with fundef unit p b.
-    exact wt_p. exact H1.
-    rewrite H2 in H1. 
-    discriminate. }
-  try (generalize (wt_instrs _ _ WT_FN pc _ H0); intros WTI).
+    exact wt_p. exact H0.
+    discriminate.
   econstructor; eauto.
   econstructor; eauto. inv WTI; auto.
-  inv WTI. rewrite <- H9. apply wt_regset_list. auto.
-- (* Itailcall *)
+  inv WTI. rewrite <- H8. apply wt_regset_list. auto.
+  (* Itailcall *)
   assert (wt_fundef fd).
-    destruct ros; simpl in H1.
+    destruct ros; simpl in H0.
     pattern fd. apply Genv.find_funct_prop with fundef unit p (rs#r).
-    exact wt_p. exact H1.
-    caseEq (Genv.find_symbol ge i); intros; rewrite H2 in H1.
+    exact wt_p. exact H0.
+    caseEq (Genv.find_symbol ge i); intros; rewrite H1 in H0.
     pattern fd. apply Genv.find_funct_ptr_prop with fundef unit p b.
-    exact wt_p. exact H1.
+    exact wt_p. exact H0.
     discriminate.
-  try (generalize (wt_instrs _ _ WT_FN pc _ H0); intros WTI).
   econstructor; eauto.
   inv WTI. apply wt_stackframes_change_sig with (fn_sig f); auto.
-  inv WTI. rewrite <- H9. apply wt_regset_list. auto.
-- (* Ibuiltin *)
+  inv WTI. rewrite <- H8. apply wt_regset_list. auto.
+  (* Ibuiltin *)
   econstructor; eauto. eapply wt_exec_Ibuiltin; eauto.
-- (* Icond *)
+  (* Icond *)
   econstructor; eauto.
-- (* Ijumptable *)
+  (* Ijumptable *)
   econstructor; eauto.
-- (* Ireturn *)
+  (* Ireturn *)
   econstructor; eauto.
   inv WTI; simpl. auto. unfold proj_sig_res; rewrite H2. auto.
-- (* internal function *)
+  (* internal function *)
   simpl in *. inv H7.
   econstructor; eauto.
   inv H2. apply wt_init_regs; auto. rewrite wt_params0. auto.
-- (* external function *)
+  (* external function *)
   econstructor; eauto. simpl.
   eapply external_call_well_typed; eauto.
-- (* return *)
+  (* return *)
   inv H2. econstructor; eauto.
   apply wt_regset_assign; auto. rewrite H11; auto.
 Qed.
 
 Lemma wt_initial_state:
-  forall S, initial_state (*SACC:*)fn_stack_requirements p S -> wt_state S.
+  forall S, initial_state fn_stack_requirements p S -> wt_state (Some Tint) S.
 Proof.
   intros. inv H. constructor. constructor. rewrite H3; auto.
   pattern f. apply Genv.find_funct_ptr_prop with fundef unit p b.
@@ -991,8 +997,9 @@ Proof.
 Qed.
 
 Lemma wt_instr_inv:
+  forall restyp,
   forall s f sp pc rs m i,
-  wt_state (State s f sp pc rs m) ->
+  wt_state restyp (State s f sp pc rs m) ->
   f.(fn_code)!pc = Some i ->
   exists env, wt_instr f env i /\ wt_regset env rs.
 Proof.
@@ -1003,3 +1010,4 @@ Qed.
 End SUBJECT_REDUCTION.
 
 
+End WITHEXTCALLS.
