common/Memory.v
@@ -8776,18 +8776,6 @@ Proof.
   destr.
 Qed.
 
-Lemma magree_push_new_stage:
-  forall m1 m2 P,
-    magree m1 m2 P ->
-    magree (push_new_stage m1) (push_new_stage m2) P.
-Proof.
-  intros m1 m2 P MI. inv MI. constructor; eauto.
-  simpl. 
-  apply stack_inject_push_new_stage.
-  eapply stack_inject_invariant_strong; eauto.
-  simpl. omega.
-Qed.
-
 Theorem magree_unrecord:
   forall m1 m2 P,
   magree m1 m2 P ->
